OCL_Normal_Form.thy
@@ -1,0 +1,244 @@
+(*  Title:       Simple OCL Semantics
+    Author:      Denis Nikiforov, December 2018
+    Maintainer:  Denis Nikiforov <denis.nikif at gmail.com>
+    License:     LGPL
+*)
+chapter \<open>OCL Expressions Normal Form\<close>
+theory OCL_Normal_Form
+  imports OCL_Typing
+begin
+
+inductive normalize
+    :: "('a :: ocl_object_model) type env \<Rightarrow> 'a expr \<Rightarrow> 'a expr \<Rightarrow> bool"
+    ("_ \<turnstile> _ \<Rrightarrow>/ _" [51,51,51] 50) and
+    normalize_call ("_ \<turnstile> _ \<Rrightarrow>\<^sub>C/ _" [51,51,51] 50)
+    where
+ LiteralN:
+  "\<Gamma> \<turnstile> Literal a \<Rrightarrow> Literal a"
+|LetN:
+  "\<Gamma> \<turnstile> init1 \<Rrightarrow> init2 \<Longrightarrow>
+   fmupd v \<tau> \<Gamma> \<turnstile> body1 \<Rrightarrow> body2 \<Longrightarrow>
+   \<Gamma> \<turnstile> Let v \<tau> init1 body1 \<Rrightarrow> Let v \<tau> init2 body2"
+|VarN:
+  "\<Gamma> \<turnstile> Var v \<Rrightarrow> Var v"
+|IfN:
+  "\<Gamma> \<turnstile> a1 \<Rrightarrow> a2 \<Longrightarrow>
+   \<Gamma> \<turnstile> b1 \<Rrightarrow> b2 \<Longrightarrow>
+   \<Gamma> \<turnstile> c1 \<Rrightarrow> c2 \<Longrightarrow>
+   \<Gamma> \<turnstile> If a1 b1 c1 \<Rrightarrow> If a1 b1 c1"
+
+|OclAnyDotCallN:
+  "\<Gamma> \<turnstile> src1 \<Rrightarrow> src2 \<Longrightarrow>
+   \<Gamma> \<turnstile> src2 : \<tau> \<Longrightarrow>
+   \<tau> \<le> OclAny[1] \<Longrightarrow>
+   (\<Gamma>, \<tau>) \<turnstile> call1 \<Rrightarrow>\<^sub>C call2 \<Longrightarrow>
+   \<Gamma> \<turnstile> Call src1 DotCall call1 \<Rrightarrow> Call src2 DotCall call2"
+|OclAnySafeDotCallN:
+  "\<Gamma> \<turnstile> src1 \<Rrightarrow> src2 \<Longrightarrow>
+   \<Gamma> \<turnstile> src2 : \<tau> \<Longrightarrow>
+   OclVoid \<le> \<tau> \<Longrightarrow>
+   \<tau> \<le> OclAny[?] \<Longrightarrow>
+   (\<Gamma>, \<tau>) \<turnstile> call1 \<Rrightarrow>\<^sub>C call2 \<Longrightarrow>
+   \<Gamma> \<turnstile> Call src1 SafeDotCall call1 \<Rrightarrow>
+       If (BinaryOperationCall src2 DotCall NotEqualOp NullLiteral)
+          (Call src2 DotCall call2)
+          NullLiteral"
+|OclAnyArrowDotCallN:
+  "\<Gamma> \<turnstile> src1 \<Rrightarrow> src2 \<Longrightarrow>
+   \<Gamma> \<turnstile> src2 : \<tau> \<Longrightarrow>
+   \<tau> \<le> OclAny[?] \<Longrightarrow>
+   (\<Gamma>, \<tau>) \<turnstile> call1 \<Rrightarrow>\<^sub>C call2 \<Longrightarrow>
+   \<Gamma> \<turnstile> Call src1 ArrowCall call1 \<Rrightarrow>
+       Call (UnaryOperationCall src2 DotCall OclAsSetOp) ArrowCall call2"
+
+|CollectionArrowCallN:
+  "\<Gamma> \<turnstile> src1 \<Rrightarrow> src2 \<Longrightarrow>
+   \<Gamma> \<turnstile> src2 : \<tau> \<Longrightarrow>
+   element_type \<tau> _ \<Longrightarrow>
+   (\<Gamma>, \<tau>) \<turnstile> call1 \<Rrightarrow>\<^sub>C call2 \<Longrightarrow>
+   \<Gamma> \<turnstile> Call src1 ArrowCall call1 \<Rrightarrow> Call src2 ArrowCall call2"
+|CollectionSafeArrowCallN:
+  "\<Gamma> \<turnstile> src1 \<Rrightarrow> src2 \<Longrightarrow>
+   \<Gamma> \<turnstile> src2 : \<tau> \<Longrightarrow>
+   element_type \<tau> \<sigma> \<Longrightarrow>
+   OclVoid \<le> \<sigma> \<Longrightarrow>
+   \<sigma> \<le> OclAny[?] \<Longrightarrow>
+   (\<Gamma>, \<tau>) \<turnstile> call1 \<Rrightarrow>\<^sub>C call2 \<Longrightarrow>
+   \<Gamma> \<turnstile> Call src1 SafeArrowCall call1 \<Rrightarrow>
+       Call (BinaryOperationCall src2 ArrowCall ExcludingOp NullLiteral) ArrowCall call2"
+|CollectionDotCallN:
+  "\<Gamma> \<turnstile> src1 \<Rrightarrow> src2 \<Longrightarrow>
+   \<Gamma> \<turnstile> src2 : \<tau> \<Longrightarrow>
+   element_type \<tau> \<sigma> \<Longrightarrow>
+   \<not> OclVoid \<le> \<sigma> \<Longrightarrow>
+   (\<Gamma>, \<tau>) \<turnstile> call1 \<Rrightarrow>\<^sub>C call2 \<Longrightarrow>
+   it = new_vname \<Gamma> \<Longrightarrow>
+   \<Gamma> \<turnstile> Call src1 DotCall call1 \<Rrightarrow> IteratorCall src2 ArrowCall CollectIter [it]
+          (Call (Var it) DotCall call2)"
+|CollectionSafeDotCallN:
+  "\<Gamma> \<turnstile> src1 \<Rrightarrow> src2 \<Longrightarrow>
+   \<Gamma> \<turnstile> src2 : \<tau> \<Longrightarrow>
+   element_type \<tau> \<sigma> \<Longrightarrow>
+   OclVoid \<le> \<sigma> \<Longrightarrow>
+   \<sigma> \<le> OclAny[?] \<Longrightarrow>
+   (\<Gamma>, \<tau>) \<turnstile> call1 \<Rrightarrow>\<^sub>C call2 \<Longrightarrow>
+   it = new_vname \<Gamma> \<Longrightarrow>
+   \<Gamma> \<turnstile> Call src1 SafeDotCall call1 \<Rrightarrow>
+      IteratorCall (BinaryOperationCall src2 ArrowCall ExcludingOp NullLiteral)
+        ArrowCall CollectIter [it]
+          (Call (Var it) DotCall call2)"
+
+|OclTypeN:
+  "(\<Gamma>, \<tau>) \<turnstile> OclType \<Rrightarrow>\<^sub>C OclType"
+|TypeOperationN:
+  "(\<Gamma>, \<tau>) \<turnstile> TypeOperation op ty \<Rrightarrow>\<^sub>C TypeOperation op ty"
+|UnaryOperationN:
+  "(\<Gamma>, \<tau>) \<turnstile> UnaryOperation op \<Rrightarrow>\<^sub>C UnaryOperation op"
+|BinaryOperationN:
+  "\<Gamma> \<turnstile> a1 \<Rrightarrow> a2 \<Longrightarrow>
+   (\<Gamma>, \<tau>) \<turnstile> BinaryOperation op a1 \<Rrightarrow>\<^sub>C BinaryOperation op a2"
+|TernaryOperationN:
+  "\<Gamma> \<turnstile> a1 \<Rrightarrow> a2 \<Longrightarrow>
+   \<Gamma> \<turnstile> b1 \<Rrightarrow> b2 \<Longrightarrow>
+   (\<Gamma>, \<tau>) \<turnstile> TernaryOperation op a1 b1 \<Rrightarrow>\<^sub>C TernaryOperation op a2 b2"
+|IterateN:
+  "element_type \<tau> \<sigma> \<Longrightarrow>
+   \<Gamma> \<turnstile> res_init1 \<Rrightarrow> res_init2 \<Longrightarrow>
+   fmadd \<Gamma> (fmap_of_list (map (\<lambda>it. (it, \<sigma>)) its)) \<turnstile>
+      Let res res_t res_init1 body1 \<Rrightarrow> Let res res_t res_init2 body2 \<Longrightarrow>
+   (\<Gamma>, \<tau>) \<turnstile> Iterate its res res_t res_init1 body1 \<Rrightarrow>\<^sub>C Iterate its res res_t res_init2 body2"
+|IteratorN:
+  "element_type \<tau> \<sigma> \<Longrightarrow>
+   fmadd \<Gamma> (fmap_of_list (map (\<lambda>it. (it, \<sigma>)) its)) \<turnstile> body1 \<Rrightarrow> body2  \<Longrightarrow>
+   (\<Gamma>, \<tau>) \<turnstile> Iterator iter its body1 \<Rrightarrow>\<^sub>C Iterator iter its body2"
+|AttributeN:
+  "(\<Gamma>, \<tau>) \<turnstile> Attribute attr \<Rrightarrow>\<^sub>C Attribute attr"
+|AssociationEndN:
+  "(\<Gamma>, \<tau>) \<turnstile> AssociationEnd role \<Rrightarrow>\<^sub>C AssociationEnd role"
+|OperationN:
+  "(\<Gamma>, \<tau>) \<turnstile> Operation op as \<Rrightarrow>\<^sub>C Operation op as"
+
+code_pred [show_modes] normalize .
+
+values "{x. (fmempty :: classes1 type env) \<turnstile>
+  (UnaryOperationCall
+    (CollectionLiteral SequenceKind [CollectionRange (IntegerLiteral 1) (IntegerLiteral 5)])
+    DotCall ToStringOp) \<Rrightarrow> x}"
+
+inductive_cases Literal_normalize [elim]: "\<Gamma> \<turnstile> Literal a \<Rrightarrow> b"
+inductive_cases Let_normalize [elim]: "\<Gamma> \<turnstile> Let v t init body \<Rrightarrow> b"
+inductive_cases Var_normalize [elim]: "\<Gamma> \<turnstile> Var v \<Rrightarrow> b"
+inductive_cases If_normalize [elim]: "\<Gamma> \<turnstile> If a b c \<Rrightarrow> d"
+inductive_cases DotCall_normalize [elim]: "\<Gamma> \<turnstile> Call src DotCall call \<Rrightarrow> b"
+inductive_cases SafeDotCall_normalize [elim]: "\<Gamma> \<turnstile> Call src SafeDotCall call \<Rrightarrow> b"
+inductive_cases ArrowCall_normalize [elim]: "\<Gamma> \<turnstile> Call src ArrowCall call \<Rrightarrow> b"
+inductive_cases SafeArrowCall_normalize [elim]: "\<Gamma> \<turnstile> Call src SafeArrowCall call \<Rrightarrow> b"
+
+inductive_cases normalize_call_elim [elim]: "(\<Gamma>, \<tau>) \<turnstile> call \<Rrightarrow>\<^sub>C b"
+inductive_cases BinaryOperation_normalize_call [elim]:
+  "(\<Gamma>, \<tau>) \<turnstile> BinaryOperation op a1 \<Rrightarrow>\<^sub>C call2"
+inductive_cases TernaryOperation_normalize_call [elim]:
+  "(\<Gamma>, \<tau>) \<turnstile> TernaryOperation op a1 b1 \<Rrightarrow>\<^sub>C call2"
+inductive_cases Iterate_normalize_call [elim]:
+  "(\<Gamma>, \<tau>) \<turnstile> Iterate its res res_t res_init1 body1 \<Rrightarrow>\<^sub>C call2"
+inductive_cases Iterator_normalize_call [elim]:
+  "(\<Gamma>, \<tau>) \<turnstile> Iterator iter its body1 \<Rrightarrow>\<^sub>C call2"
+
+lemma any_has_not_element_type:
+  "\<tau> \<le> OclAny[?] \<Longrightarrow> element_type \<tau> \<sigma> \<Longrightarrow> False"
+  by (erule element_type.cases; auto)
+
+lemma
+  normalize_det: "\<Gamma> \<turnstile> expr \<Rrightarrow> expr1 \<Longrightarrow> \<Gamma> \<turnstile> expr \<Rrightarrow> expr2 \<Longrightarrow> expr1 = expr2" and
+  normalize_call_det: "\<Gamma>1 \<turnstile> call \<Rrightarrow>\<^sub>C call1 \<Longrightarrow> \<Gamma>1 \<turnstile> call \<Rrightarrow>\<^sub>C call2 \<Longrightarrow> call1 = call2"
+  for \<Gamma> :: "('a :: ocl_object_model) type env"
+  and \<Gamma>1 :: "('a :: ocl_object_model) type env \<times> 'a type"
+proof (induct \<Gamma> expr expr1 and \<Gamma>1 call call1
+       arbitrary: expr2 and call2
+       rule: normalize_normalize_call.inducts)
+  case (LiteralN \<Gamma> a) thus ?case by auto
+next
+  case (LetN \<Gamma> init1 init2 v \<tau> body1 body2) thus ?case by blast
+next
+  case (VarN \<Gamma> v) thus ?case by auto
+next
+  case (IfN \<Gamma> a1 a2 b1 b2 c1 c2) thus ?case by auto
+next
+  case (OclAnyDotCallN \<Gamma> src1 src2 \<tau> call1 call2) show ?case
+    apply (insert OclAnyDotCallN.prems)
+    apply (erule DotCall_normalize)
+    apply (metis OclAnyDotCallN.hyps(2) OclAnyDotCallN.hyps(3) OclAnyDotCallN.hyps(6) typing_det)
+    by (metis OclAnyDotCallN.hyps(2) OclAnyDotCallN.hyps(3) OclAnyDotCallN.hyps(4) any_has_not_element_type type_less_eq_x_Optional_intro(2) typing_det)
+next
+  case (OclAnySafeDotCallN \<Gamma> src1 src2 \<tau> call1 call2) show ?case
+    apply (insert OclAnySafeDotCallN.prems)
+    apply (erule SafeDotCall_normalize)
+    apply (metis OclAnySafeDotCallN.hyps(2) OclAnySafeDotCallN.hyps(3) OclAnySafeDotCallN.hyps(7) typing_det)
+    by (metis OclAnySafeDotCallN.hyps(2) OclAnySafeDotCallN.hyps(3) OclAnySafeDotCallN.hyps(5) any_has_not_element_type typing_det)
+next
+  case (OclAnyArrowDotCallN \<Gamma> src1 src2 \<tau> call1 call2) show ?case
+    apply (insert OclAnyArrowDotCallN.prems)
+    apply (erule ArrowCall_normalize)
+    apply (metis OclAnyArrowDotCallN.hyps(2) OclAnyArrowDotCallN.hyps(3) OclAnyArrowDotCallN.hyps(6) typing_det)
+    by (metis OclAnyArrowDotCallN.hyps(2) OclAnyArrowDotCallN.hyps(3) OclAnyArrowDotCallN.hyps(4) any_has_not_element_type typing_det)
+next
+  case (CollectionArrowCallN \<Gamma> src1 src2 \<tau> call1 call2 uu) show ?case
+    apply (insert CollectionArrowCallN.prems)
+    apply (erule ArrowCall_normalize)
+    apply (metis CollectionArrowCallN.hyps(2) CollectionArrowCallN.hyps(3) CollectionArrowCallN.hyps(4) any_has_not_element_type typing_det)
+    using CollectionArrowCallN.hyps(2) CollectionArrowCallN.hyps(3) CollectionArrowCallN.hyps(6) typing_det by fastforce
+next
+  case (CollectionSafeArrowCallN \<Gamma> src1 src2 \<tau> call1 call2 \<sigma>) show ?case
+    apply (insert CollectionSafeArrowCallN.prems)
+    apply (erule SafeArrowCall_normalize)
+    by (metis CollectionSafeArrowCallN.hyps(2) CollectionSafeArrowCallN.hyps(3) CollectionSafeArrowCallN.hyps(8) comp_eq_dest_lhs typing_det)
+next
+  case (CollectionDotCallN \<Gamma> src1 src2 \<tau> call1 call2 \<sigma> it) show ?case
+    apply (insert CollectionDotCallN.prems)
+    apply (erule DotCall_normalize)
+    apply (metis CollectionDotCallN.hyps(2) CollectionDotCallN.hyps(3) CollectionDotCallN.hyps(4) any_has_not_element_type type_less_eq_x_Optional_intro(2) typing_det)
+    using CollectionDotCallN.hyps(2) CollectionDotCallN.hyps(3) CollectionDotCallN.hyps(7) CollectionDotCallN.hyps(8) typing_det by fastforce
+next
+  case (CollectionSafeDotCallN \<Gamma> src1 src2 \<tau> call1 call2 \<sigma> it) show ?case
+    apply (insert CollectionSafeDotCallN.prems)
+    apply (erule SafeDotCall_normalize)
+    apply (metis CollectionSafeDotCallN.hyps(2) CollectionSafeDotCallN.hyps(3) CollectionSafeDotCallN.hyps(4) any_has_not_element_type typing_det)
+    by (metis CollectionSafeDotCallN.hyps(2) CollectionSafeDotCallN.hyps(3) CollectionSafeDotCallN.hyps(8) CollectionSafeDotCallN.hyps(9) comp_eq_dest_lhs typing_det)
+next
+  case (OclTypeN \<Gamma> \<tau>) thus ?case by auto
+next
+  case (TypeOperationN \<Gamma> \<tau> op ty) thus ?case by auto
+next
+  case (UnaryOperationN \<Gamma> \<tau> op) thus ?case by auto
+next
+  case (BinaryOperationN \<Gamma> a1 a2 \<tau> op) show ?case
+    apply (insert BinaryOperationN.prems)
+    apply (erule BinaryOperation_normalize_call)
+    by (simp add: BinaryOperationN.hyps(2))
+next
+  case (TernaryOperationN \<Gamma> a1 a2 b1 b2 \<tau> op) show ?case
+    apply (insert TernaryOperationN.prems)
+    apply (erule TernaryOperation_normalize_call)
+    by (simp add: TernaryOperationN.hyps(2) TernaryOperationN.hyps(4))
+next
+  case (IterateN \<tau> \<sigma> \<Gamma> res_init1 res_init2 its res res_t body1 body2)
+  show ?case
+    apply (insert IterateN.prems)
+    apply (erule Iterate_normalize_call)
+    using IterateN.hyps(1) IterateN.hyps(5) element_type_det by blast
+next
+  case (IteratorN \<tau> \<sigma> \<Gamma> its body1 body2 iter)
+  show ?case
+    apply (insert IteratorN.prems)
+    apply (erule Iterator_normalize_call)
+    using IteratorN.hyps(1) IteratorN.hyps(3) element_type_det by auto
+next
+  case (AttributeN \<Gamma> \<tau> attr) thus ?case by auto
+next
+  case (AssociationEndN \<Gamma> \<tau> role) thus ?case by auto
+next
+  case (OperationN \<Gamma> \<tau> op as) thus ?case by auto
+qed
+
+
+end
