Preliminaries.thy
@@ -4,7 +4,7 @@
     License:     LGPL
 *)
 theory Preliminaries
-  imports Transitive_Closure_Ext Finite_Map_Ext Tuple
+  imports Transitive_Closure_Ext Finite_Map_Ext Tuple Object_Model
 begin
 
 end
